context

Logic/Logic/Context.lean
@@ -7,53 +7,53 @@ namespace System
 
 variable (F : Type*) [LogicalConnective F] [DecidableEq F] {S : Type*} [System F S]
 
-structure Context (𝓢 : S) where
+structure FiniteContext (𝓢 : S) where
   ctx : List F
 
 variable {F}
 
-namespace Context
+namespace FiniteContext
 
 variable {𝓢 : S}
 
-instance : Coe (List F) (Context F 𝓢) := ⟨mk⟩
+instance : Coe (List F) (FiniteContext F 𝓢) := ⟨mk⟩
 
-abbrev conj (Γ : Context F 𝓢) : F := Γ.ctx.conj
+abbrev conj (Γ : FiniteContext F 𝓢) : F := Γ.ctx.conj
 
-abbrev disj (Γ : Context F 𝓢) : F := Γ.ctx.disj
+abbrev disj (Γ : FiniteContext F 𝓢) : F := Γ.ctx.disj
 
-instance : EmptyCollection (Context F 𝓢) := ⟨⟨[]⟩⟩
+instance : EmptyCollection (FiniteContext F 𝓢) := ⟨⟨[]⟩⟩
 
-instance : Membership F (Context F 𝓢) := ⟨(· ∈ ·.ctx)⟩
+instance : Membership F (FiniteContext F 𝓢) := ⟨(· ∈ ·.ctx)⟩
 
-instance : HasSubset (Context F 𝓢) := ⟨(·.ctx ⊆ ·.ctx)⟩
+instance : HasSubset (FiniteContext F 𝓢) := ⟨(·.ctx ⊆ ·.ctx)⟩
 
-instance : Cons F (Context F 𝓢) := ⟨(· :: ·.ctx)⟩
+instance : Cons F (FiniteContext F 𝓢) := ⟨(· :: ·.ctx)⟩
 
-lemma mem_def {p : F} {Γ : Context F 𝓢} : p ∈ Γ ↔ p ∈ Γ.ctx := iff_of_eq rfl
+lemma mem_def {p : F} {Γ : FiniteContext F 𝓢} : p ∈ Γ ↔ p ∈ Γ.ctx := iff_of_eq rfl
 
-@[simp] lemma coe_subset_coe_iff {Γ Δ : List F} : (Γ : Context F 𝓢) ⊆ Δ ↔ Γ ⊆ Δ := iff_of_eq rfl
+@[simp] lemma coe_subset_coe_iff {Γ Δ : List F} : (Γ : FiniteContext F 𝓢) ⊆ Δ ↔ Γ ⊆ Δ := iff_of_eq rfl
 
-@[simp] lemma mem_coe_iff {p : F} {Γ : List F} : p ∈ (Γ : Context F 𝓢) ↔ p ∈ Γ := iff_of_eq rfl
+@[simp] lemma mem_coe_iff {p : F} {Γ : List F} : p ∈ (Γ : FiniteContext F 𝓢) ↔ p ∈ Γ := iff_of_eq rfl
 
-@[simp] lemma not_mem_empty (p : F) : ¬p ∈ (∅ : Context F 𝓢) := by simp [EmptyCollection.emptyCollection]
+@[simp] lemma not_mem_empty (p : F) : ¬p ∈ (∅ : FiniteContext F 𝓢) := by simp [EmptyCollection.emptyCollection]
 
-instance : Collection F (Context F 𝓢) where
+instance : Collection F (FiniteContext F 𝓢) where
   subset_iff := List.subset_def
   not_mem_empty := by simp
   mem_cons_iff := by simp [Cons.cons, mem_def]
 
-instance (𝓢 : S) : System F (Context F 𝓢) := ⟨(𝓢 ⊢ ·.conj ⟶ ·)⟩
+instance (𝓢 : S) : System F (FiniteContext F 𝓢) := ⟨(𝓢 ⊢ ·.conj ⟶ ·)⟩
 
-abbrev Prf (𝓢 : S) (Γ : List F) (p : F) := (Γ : Context F 𝓢) ⊢ p
+abbrev Prf (𝓢 : S) (Γ : List F) (p : F) := (Γ : FiniteContext F 𝓢) ⊢ p
 
-abbrev Provable (𝓢 : S) (Γ : List F) (p : F) := (Γ : Context F 𝓢) ⊢! p
+abbrev Provable (𝓢 : S) (Γ : List F) (p : F) := (Γ : FiniteContext F 𝓢) ⊢! p
 
-local notation Γ:45 " ⊢[" 𝓢 "] " p:46 => Prf 𝓢 Γ p
+notation Γ:45 " ⊢[" 𝓢 "] " p:46 => Prf 𝓢 Γ p
 
-local notation Γ:45 " ⊢[" 𝓢 "]! " p:46 => Provable 𝓢 Γ p
+notation Γ:45 " ⊢[" 𝓢 "]! " p:46 => Provable 𝓢 Γ p
 
-lemma system_def (Γ : Context F 𝓢) (p : F) : (Γ ⊢ p) = (𝓢 ⊢ Γ.conj ⟶ p) := rfl
+lemma system_def (Γ : FiniteContext F 𝓢) (p : F) : (Γ ⊢ p) = (𝓢 ⊢ Γ.conj ⟶ p) := rfl
 
 def of {Γ : List F} {p : F} (b : 𝓢 ⊢ Γ.conj ⟶ p) : Γ ⊢[𝓢] p := b
 
@@ -65,7 +65,7 @@ section minimal
 
 variable [Minimal 𝓢] {Γ Δ E : List F}
 
-instance : Axiomatized (Context F 𝓢) where
+instance : Axiomatized (FiniteContext F 𝓢) where
   prfAxm := fun _ _ hp ↦ generalConj hp
   weakening := fun H b ↦ impTrans (conjImplyConj H) b
 
@@ -84,7 +84,7 @@ def emptyPrf {p : F} : [] ⊢[𝓢] p → 𝓢 ⊢ p := fun b ↦ b ⨀ verum
 def provable_iff_provable {p : F} : 𝓢 ⊢! p ↔ [] ⊢[𝓢]! p :=
   ⟨fun b ↦ ⟨of' b.some _⟩, fun b ↦ ⟨emptyPrf b.some⟩⟩
 
-instance minimal (Γ : Context F 𝓢) : Minimal Γ where
+instance minimal (Γ : FiniteContext F 𝓢) : Minimal Γ where
   mdp := mdp₁
   verum := of' verum _
   imply₁ := fun _ _ ↦ of' imply₁ _
@@ -105,27 +105,85 @@ def deductInv {p q : F} {Γ : List F} : Γ ⊢[𝓢] p ⟶ q → (p :: Γ) ⊢[�
 lemma deduct_iff {p q : F} {Γ : List F} : Γ ⊢[𝓢]! p ⟶ q ↔ (p :: Γ) ⊢[𝓢]! q :=
   ⟨fun h ↦ ⟨deductInv h.some⟩, fun h ↦ ⟨deduct h.some⟩⟩
 
-instance deduction : Deduction (Context F 𝓢) where
+instance deduction : Deduction (FiniteContext F 𝓢) where
   ofInsert := deduct
   inv := deductInv
 
-instance hasEFQ [HasEFQ 𝓢] (Γ : Context F 𝓢) : HasEFQ Γ := ⟨fun _ ↦ of <| dhyp Γ.conj efq⟩
+instance hasEFQ [HasEFQ 𝓢] (Γ : FiniteContext F 𝓢) : HasEFQ Γ := ⟨fun _ ↦ of <| dhyp Γ.conj efq⟩
 
-instance hasWeakLEM [HasWeakLEM 𝓢] (Γ : Context F 𝓢) : HasWeakLEM Γ := ⟨fun p ↦ of <| dhyp Γ.conj (HasWeakLEM.wlem p)⟩
+instance hasWeakLEM [HasWeakLEM 𝓢] (Γ : FiniteContext F 𝓢) : HasWeakLEM Γ := ⟨fun p ↦ of <| dhyp Γ.conj (HasWeakLEM.wlem p)⟩
 
-instance dummett [Dummett 𝓢] (Γ : Context F 𝓢) : Dummett Γ := ⟨fun p q ↦ of <| dhyp Γ.conj (Dummett.dummett p q)⟩
+instance dummett [Dummett 𝓢] (Γ : FiniteContext F 𝓢) : Dummett Γ := ⟨fun p q ↦ of <| dhyp Γ.conj (Dummett.dummett p q)⟩
 
-instance hasDNE [HasDNE 𝓢] (Γ : Context F 𝓢) : HasDNE Γ := ⟨fun p ↦ of <| dhyp Γ.conj (HasDNE.dne p)⟩
+instance hasDNE [HasDNE 𝓢] (Γ : FiniteContext F 𝓢) : HasDNE Γ := ⟨fun p ↦ of <| dhyp Γ.conj (HasDNE.dne p)⟩
 
 end minimal
 
-instance intuitionistic [Intuitionistic 𝓢] (Γ : Context F 𝓢) : Intuitionistic Γ where
+instance intuitionistic [Intuitionistic 𝓢] (Γ : FiniteContext F 𝓢) : Intuitionistic Γ where
 
-instance weakLEM [WeakLEM 𝓢] (Γ : Context F 𝓢) : WeakLEM Γ where
+instance weakLEM [WeakLEM 𝓢] (Γ : FiniteContext F 𝓢) : WeakLEM Γ where
 
-instance gd [GD 𝓢] (Γ : Context F 𝓢) : GD Γ where
+instance gd [GD 𝓢] (Γ : FiniteContext F 𝓢) : GD Γ where
 
-instance classical [Classical 𝓢] (Γ : Context F 𝓢) : Classical Γ where
+instance classical [Classical 𝓢] (Γ : FiniteContext F 𝓢) : Classical Γ where
+
+end FiniteContext
+
+variable (F)
+
+structure Context (𝓢 : S) where
+  ctx : Set F
+
+variable {F}
+
+namespace Context
+
+variable {𝓢 : S}
+
+instance : Coe (Set F) (Context F 𝓢) := ⟨mk⟩
+
+instance : EmptyCollection (Context F 𝓢) := ⟨⟨∅⟩⟩
+
+instance : Membership F (Context F 𝓢) := ⟨(· ∈ ·.ctx)⟩
+
+instance : HasSubset (Context F 𝓢) := ⟨(·.ctx ⊆ ·.ctx)⟩
+
+instance : Cons F (Context F 𝓢) := ⟨(⟨insert · ·.ctx⟩)⟩
+
+lemma mem_def {p : F} {Γ : Context F 𝓢} : p ∈ Γ ↔ p ∈ Γ.ctx := iff_of_eq rfl
+
+@[simp] lemma coe_subset_coe_iff {Γ Δ : Set F} : (Γ : Context F 𝓢) ⊆ Δ ↔ Γ ⊆ Δ := iff_of_eq rfl
+
+@[simp] lemma mem_coe_iff {p : F} {Γ : Set F} : p ∈ (Γ : Context F 𝓢) ↔ p ∈ Γ := iff_of_eq rfl
+
+@[simp] lemma not_mem_empty (p : F) : ¬p ∈ (∅ : Context F 𝓢) := by simp [EmptyCollection.emptyCollection, Set.mem_def]
+
+instance : Collection F (Context F 𝓢) where
+  subset_iff := by rintro ⟨s⟩ ⟨u⟩; simp [Set.subset_def]
+  not_mem_empty := by simp
+  mem_cons_iff := by simp [Cons.cons, mem_def]
+
+structure Proof (Γ : Context F 𝓢) (p : F) where
+  ctx : List F
+  subset : ∀ q ∈ ctx, q ∈ Γ
+  prf : ctx ⊢[𝓢] p
+
+instance (𝓢 : S) : System F (Context F 𝓢) := ⟨Proof⟩
+
+variable (𝓢)
+
+abbrev Prf (Γ : Set F) (p : F) : Type _ := (Γ : Context F 𝓢) ⊢ p
+
+abbrev Provable (Γ : Set F) (p : F) : Prop := (Γ : Context F 𝓢) ⊢! p
+
+notation Γ:45 " *⊢[" 𝓢 "] " p:46 => Prf 𝓢 Γ p
+
+notation Γ:45 " *⊢[" 𝓢 "]! " p:46 => Provable 𝓢 Γ p
+
+variable {𝓢}
+
+lemma provable_iff {p : F} : Γ *⊢[𝓢]! p ↔ ∃ Δ : List F, (∀ q ∈ Δ, q ∈ Γ) ∧ Δ ⊢[𝓢]! p :=
+  ⟨by rintro ⟨⟨Δ, h, b⟩⟩; exact ⟨Δ, h, ⟨b⟩⟩, by rintro ⟨Δ, h, ⟨d⟩⟩; exact ⟨⟨Δ, h, d⟩⟩⟩
 
 end Context
 
